src/StatDb/StatDbAPI.v
@@ -33,7 +33,7 @@ Module Type StatDbAPI.
 
   Axiom add_ok : forall v, prog_spec (add_spec v) (add v) recover abstr.
   Axiom mean_ok : prog_spec mean_spec mean recover abstr.
-  Axiom recover_noop : rec_noop recover abstr (@no_crash _).
+  Axiom recover_noop : rec_noop recover abstr no_crash.
 
   Hint Resolve add_ok.
   Hint Resolve mean_ok.
